normalform.v
@@ -1,0 +1,298 @@
+From WR Require Import syntax join imports.
+
+Fixpoint ne (a : tm) :=
+  match a with
+  | var_tm _ => true
+  | tApp a b => ne a && nf b
+  | tAbs _ => false
+  | tPi A B => false
+  | tVoid => false
+  | tJ t a b p => nf t && nf a && nf b && ne p
+  | tUniv _ => false
+  | tTrue => false
+  | tFalse => false
+  | tIf a b c => ne a && nf b && nf c
+  | tBool => false
+  | tEq a b A => false
+  | tRefl => false
+  end
+with nf (a : tm) :=
+  match a with
+  | var_tm _ => true
+  | tApp a b => ne a && nf b
+  | tAbs a => nf a
+  | tPi A B => nf A && nf B
+  | tVoid => true
+  | tJ t a b p => nf t && nf a && nf b && ne p
+  | tUniv _ => true
+  | tTrue => true
+  | tFalse => true
+  | tIf a b c => ne a && nf b && nf c
+  | tBool => true
+  | tEq a b A => nf a && nf b && nf A
+  | tRefl => true
+  end.
+
+Definition wn (a : tm) := exists b, Pars a b /\ nf b.
+Definition wne (a : tm) := exists b, Pars a b /\ ne b.
+
+Lemma bool_val_nf v : is_bool_val v -> nf v.
+Proof. case : v =>// _; hauto lq:on unfold:nf inv:Par. Qed.
+
+Lemma ne_nf (a : tm) : ne a -> nf a.
+Proof. elim : a =>//; hauto q:on unfold:nf inv:Par. Qed.
+
+Lemma ne_nf_renaming (a : tm) :
+  forall (ξ : nat -> nat),
+    (ne a <-> ne (ren_tm ξ a)) /\ (nf a <-> nf (ren_tm ξ a)).
+Proof.
+  elim : a; solve [auto; hauto b:on].
+Qed.
+
+Create HintDb nfne.
+Lemma nf_ne_preservation a b (h : Par a b) : (nf a ==> nf b) /\ (ne a ==> ne b).
+Proof.
+  elim : a b / h => //; hauto lqb:on depth:2.
+Qed.
+
+Lemma nf_preservation : forall a b, Par a b -> nf a -> nf b.
+Proof. sfirstorder use:nf_ne_preservation b:on. Qed.
+
+Lemma ne_preservation : forall a b, Par a b -> ne a -> ne b.
+Proof. sfirstorder use:nf_ne_preservation b:on. Qed.
+
+Lemma nf_wn v : nf v -> wn v.
+Proof. sfirstorder ctrs:rtc. Qed.
+
+Lemma wne_wn a : wne a -> wn a.
+Proof. sfirstorder use:ne_nf. Qed.
+
+#[export]Hint Resolve nf_wn bool_val_nf ne_nf wne_wn ne_preservation nf_preservation : nfne.
+
+
+Lemma Par_antirenaming (a b0 : tm) (ξ : nat -> nat)
+  (h : Par (ren_tm ξ a) b0) : exists b, Par a b /\ b0 = ren_tm ξ b.
+Proof.
+  move E : (ren_tm ξ a) h => a0 h.
+  move : a ξ E.
+  elim : a0 b0 / h.
+  - move => + []//. eauto with par.
+  - move => + []//. eauto with par.
+  - move => []//. eauto with par.
+  - move => A0 A1 B0 B1 h0 ih0 h1 ih1 [] // /=.
+    hauto lq:on ctrs:Par.
+  - move => a0 a1 h ih [] // a ξ [] ?.
+    hauto lq:on ctrs:Par.
+  - move => a0 a1 b0 b1  + + + + []//.
+    hauto q:on ctrs:Par.
+  - move => a a0 b0- b1 ha iha hb ihb []// []// t t0 ξ [] *. subst.
+    specialize iha with (1 := eq_refl).
+    specialize ihb with (1 := eq_refl).
+    move : iha => [a [? ?]]. subst.
+    move : ihb => [b [? ?]]. subst.
+    exists (subst_tm (b..) a).
+    split; last by asimpl.
+    hauto lq:on ctrs:Par.
+  - hauto q:on ctrs:Par inv:tm.
+  - hauto q:on ctrs:Par inv:tm.
+  - move => > ++++++ [] //.
+    hauto q:on ctrs:Par.
+  - move => b0 b1 c0 h ih []// []// t0 t1 ξ [].
+    hauto lq:on ctrs:Par.
+  - move => b0 b1 c0 h ih []// []// t0 t1 ξ [].
+    hauto lq:on ctrs:Par.
+  - hauto inv:tm q:on ctrs:Par.
+  - hauto inv:tm q:on ctrs:Par.
+  - move => a0 b0 A0 a1 b1 A1 h ih h0 ih0 h1 ih1 []//.
+    hauto q:on ctrs:Par.
+  - move => t0 a0 b0 p0 t1 a1 b1 p1 ++++++++[]//.
+    hauto q:on ctrs:Par.
+  - move => t0 a b t1 ++[]//+++[]//.
+    hauto q:on ctrs:Par.
+Qed.
+
+Lemma Pars_antirenaming (a b0 : tm) (ξ : nat -> nat)
+  (h : Pars (ren_tm ξ a) b0) : exists b, b0 = ren_tm ξ b /\ Pars a b.
+Proof.
+  move E :  (ren_tm ξ a) h => a0 h.
+  move : a E.
+  elim : a0 b0 / h.
+  - hauto lq:on ctrs:rtc.
+  - move => a b c h0 h ih a0 ?. subst.
+    move /Par_antirenaming : h0.
+    hauto lq:on ctrs:rtc, eq.
+Qed.
+
+Lemma wn_antirenaming a (ξ : nat -> nat) : wn (ren_tm ξ a) -> wn a.
+Proof.
+  rewrite /wn.
+  move => [v [rv nfv]].
+  move /Pars_antirenaming : rv => [b [hb ?]]. subst.
+  sfirstorder use:ne_nf_renaming.
+Qed.
+
+#[local]Ltac solve_s_rec :=
+  move => *; eapply rtc_l; eauto;
+  hauto lq:on ctrs:Par use:Par_refl.
+
+Lemma S_AppLR (a a0 b b0 : tm) :
+  Pars a a0 ->
+  Pars b b0 ->
+  Pars (tApp a b) (tApp a0 b0).
+Proof.
+  move => h. move :  b b0.
+  elim : a a0 / h.
+  - move => a a0 b h.
+    elim : a0 b / h.
+    + auto using rtc_refl.
+    + solve_s_rec.
+  - solve_s_rec.
+Qed.
+
+Lemma S_If a0 a1 : forall b0 b1 c0 c1,
+    Pars a0 a1 ->
+    Pars b0 b1 ->
+    Pars c0 c1 ->
+    Pars (tIf a0 b0 c0) (tIf a1 b1 c1).
+Proof.
+  move => + + + + h.
+  elim : a0 a1 /h.
+  - move => + b0 b1 + + h.
+    elim : b0 b1 /h.
+    + move => + + c0 c1 h.
+      elim : c0 c1 /h.
+      * auto using rtc_refl.
+      * solve_s_rec.
+    + solve_s_rec.
+  - solve_s_rec.
+Qed.
+
+Lemma S_J t0 t1 : forall a0 a1 b0 b1 p0 p1,
+    Pars t0 t1 ->
+    Pars a0 a1 ->
+    Pars b0 b1 ->
+    Pars p0 p1 ->
+    Pars (tJ t0 a0 b0 p0) (tJ t1 a1 b1 p1).
+Proof.
+  move => + + + + + + h.
+  elim : t0 t1 /h; last by solve_s_rec.
+  move => + a0 a1 + +  + + h.
+  elim : a0 a1 /h; last by solve_s_rec.
+  move => + + b0 b1 + + h.
+  elim : b0 b1 /h; last by solve_s_rec.
+  move => + + + p0 p1 h.
+  elim : p0 p1 / h; last by solve_s_rec.
+  auto using rtc_refl.
+Qed.
+
+Lemma wne_j (t a b p : tm) :
+  wn t -> wn a -> wn b -> wne p -> wne (tJ t a b p).
+Proof.
+  move => [t0 [? ?]] [a0 [? ?]] [b0 [? ?]] [p0 [? ?]].
+  exists (tJ t0 a0 b0 p0).
+  hauto lq:on b:on use:S_J.
+Qed.
+
+Lemma wne_if (a b c : tm) :
+  wne a -> wn b -> wn c -> wne (tIf a b c).
+Proof.
+  move => [a0 [? ?]] [b0 [? ?]] [c0 [? ?]].
+  exists (tIf a0 b0 c0).
+  qauto l:on use:S_If b:on.
+Qed.
+
+Lemma wne_app (a b : tm) :
+  wne a -> wn b -> wne (tApp a b).
+Proof.
+  move => [a0 [? ?]] [b0 [? ?]].
+  exists (tApp a0 b0).
+  hauto b:on use:S_AppLR.
+Qed.
+
+Lemma S_Pi (a a0 b b0 : tm) :
+  Pars a a0 ->
+  Pars b b0 ->
+  Pars (tPi a b) (tPi a0 b0).
+Proof.
+  move => h.
+  move : b b0.
+  elim : a a0/h.
+  - move => + b b0 h.
+    elim : b b0/h.
+    + auto using rtc_refl.
+    + solve_s_rec.
+  - solve_s_rec.
+Qed.
+
+Lemma S_Abs (a b : tm)
+  (h : Pars a b) :
+  Pars (tAbs a) (tAbs b).
+Proof. elim : a b /h; hauto lq:on ctrs:Par,rtc. Qed.
+
+Lemma wn_abs (a : tm) (h : wn a) : wn (tAbs a).
+Proof.
+  move : h => [v [? ?]].
+  exists (tAbs v).
+  eauto using S_Abs.
+Qed.
+
+Lemma wn_pi A B : wn A -> wn B -> wn (tPi A B).
+Proof.
+  move => [A0 [? ?]] [B0 [? ?]].
+  exists (tPi A0 B0).
+  hauto lqb:on use:S_Pi.
+Qed.
+
+Lemma S_Eq a0 a1 b0 b1 A0 A1 :
+  Pars a0 a1 ->
+  Pars b0 b1 ->
+  Pars A0 A1 ->
+  Pars (tEq a0 b0 A0) (tEq a1 b1 A1).
+Proof.
+  move => h.
+  move : b0 b1 A0 A1.
+  elim : a0 a1 /h.
+  - move => + b0 b1 + + h.
+    elim : b0 b1 /h.
+    + move => + + A0 A1 h.
+      elim : A0 A1 /h.
+      * auto using rtc_refl.
+      * solve_s_rec.
+    + solve_s_rec.
+  - solve_s_rec.
+Qed.
+
+Lemma wn_eq a b A : wn a -> wn b -> wn A -> wn (tEq a b A).
+Proof.
+  rewrite /wn.
+  move => [va [? ?]] [vb [? ?]] [vA [? ?]].
+  exists (tEq va vb vA).
+  split.
+  - by apply S_Eq.
+  - hauto lqb:on.
+Qed.
+
+Lemma ext_wn (a : tm) i :
+    wn (tApp a (var_tm i)) ->
+    wn a.
+Proof.
+  move E : (tApp a (var_tm i)) => a0 [v [hr hv]].
+  move : a E.
+  move : hv.
+  elim : a0 v / hr.
+  - hauto q:on inv:tm ctrs:rtc b:on db: nfne.
+  - move => a0 a1 a2 hr0 hr1 ih hnfa2.
+    move /(_ hnfa2) in ih.
+    move => a.
+    case : a0 hr0=>// => b0 b1.
+    elim /Par_inv=>//.
+    + hauto q:on inv:Par ctrs:rtc b:on.
+    + move => ? a0 a3 b2 b3 ? ? [? ?] ? [? ?]. subst.
+      have ? : b3 = var_tm i by hauto lq:on inv:Par. subst.
+      suff : wn (tAbs a3) by hauto lq:on ctrs:Par, rtc unfold:wn.
+      have : wn (subst_tm ((var_tm i) ..) a3) by sfirstorder.
+      replace (subst_tm ((var_tm i) ..) a3) with (ren_tm (i..) a3).
+      move /wn_antirenaming.
+      by apply : wn_abs.
+      substify. by asimpl.
+Qed.
